WIP, it's a mess

ArkLib/OracleReduction/Cast.lean
@@ -4,7 +4,7 @@ Released under Apache 2.0 license as described in the file LICENSE.
 Authors: Quang Dao
 -/
 
-import ArkLib.OracleReduction.Security.Basic
+import ArkLib.OracleReduction.Security.RoundByRound
 
 /-!
   # Casting for structures of oracle reductions
@@ -15,12 +15,16 @@ import ArkLib.OracleReduction.Security.Basic
   - `(Oracle)Prover`
   - `(Oracle)Verifier`
   - `(Oracle)Reduction`
+
+  We also show that casting preserves execution (up to casting of the transcripts) and thus security
+  properties.
 -/
 
-
-namespace ProtocolSpec
+open OracleComp
 
 variable {n₁ n₂ : ℕ} (hn : n₁ = n₂)
+
+namespace ProtocolSpec
 
 /-! ### Casting Protocol Specifications -/
 
@@ -45,7 +49,7 @@ theorem cast_eq_dcast {h : n₁ = n₂} {pSpec : ProtocolSpec n₁} :
 variable {pSpec₁ : ProtocolSpec n₁} {pSpec₂ : ProtocolSpec n₂}
 
 @[simp]
-theorem cast_idx (hSpec : pSpec₁.cast hn = pSpec₂) {i : Fin n₁} :
+theorem cast_idx {hn} (hSpec : pSpec₁.cast hn = pSpec₂) {i : Fin n₁} :
     pSpec₂ (Fin.cast hn i) = pSpec₁ i := by
   simp [← hSpec, ProtocolSpec.cast]
 
@@ -85,11 +89,18 @@ end MessageIdx
 
 namespace Message
 
+variable {hn}
+
 @[simp]
-theorem cast_idx {i : MessageIdx pSpec₂} :
+theorem cast_idx_symm {i : MessageIdx pSpec₂} :
     pSpec₁.Message (i.cast hn.symm (cast_symm hSpec)) = pSpec₂.Message i := by
   simp [MessageIdx.cast]
-  exact congrArg Prod.snd (cast_idx_symm hSpec)
+  exact congrArg Prod.snd (ProtocolSpec.cast_idx_symm hSpec)
+
+theorem cast_idx {i : MessageIdx pSpec₁} :
+    pSpec₂.Message (i.cast hn hSpec) = pSpec₁.Message i := by
+  simp [MessageIdx.cast]
+  exact congrArg Prod.snd <| (ProtocolSpec.cast_idx hSpec)
 
 instance [inst : ∀ i, OracleInterface (pSpec₁.Message i)] :
     ∀ i, OracleInterface ((pSpec₁.cast hn).Message i) :=
@@ -121,11 +132,23 @@ theorem cast_eq_dcast₂ {hn} {hSpec : pSpec₁.cast hn = pSpec₂} {i : Challen
 
 end ChallengeIdx
 
+namespace Challenge
+
+variable {hn}
+
 @[simp]
-theorem Challenge.cast_idx {i : ChallengeIdx pSpec₂} :
+theorem cast_idx {i : ChallengeIdx pSpec₁} :
+    pSpec₂.Challenge (i.cast hn hSpec) = pSpec₁.Challenge i := by
+  simp [ChallengeIdx.cast]
+  exact congrArg Prod.snd <| (ProtocolSpec.cast_idx hSpec)
+
+@[simp]
+theorem cast_idx_symm {i : ChallengeIdx pSpec₂} :
     pSpec₁.Challenge (i.cast hn.symm (cast_symm hSpec)) = pSpec₂.Challenge i := by
   simp [ChallengeIdx.cast]
-  exact congrArg Prod.snd (cast_idx_symm hSpec)
+  exact congrArg Prod.snd (ProtocolSpec.cast_idx_symm hSpec)
+
+end Challenge
 
 variable {k : Fin (n₁ + 1)} {l : Fin (n₂ + 1)}
 
@@ -139,6 +162,8 @@ protected def cast (hIdx : k.val = l.val) (hSpec : pSpec₁.cast hn = pSpec₂)
 
 @[simp]
 theorem cast_id : Transcript.cast rfl rfl rfl = (id : pSpec₁.Transcript k → _) := rfl
+
+variable {hn} (hIdx : k.val = l.val) (hSpec : pSpec₁.cast hn = pSpec₂)
 
 instance instDCast₃ : DCast₃ Nat (fun n => Fin (n + 1)) (fun n _ => ProtocolSpec n)
     (fun _ k pSpec => pSpec.Transcript k) where
@@ -198,10 +223,10 @@ protected def cast (P : Prover oSpec StmtIn WitIn StmtOut WitOut pSpec₁) :
   input := P.input
   sendMessage := fun i st => do
     let ⟨msg, newSt⟩ ← P.sendMessage (i.cast hn.symm (cast_symm hSpec)) st
-    return ⟨(Message.cast_idx hn hSpec) ▸ msg, newSt⟩
+    return ⟨(Message.cast_idx_symm hSpec) ▸ msg, newSt⟩
   receiveChallenge := fun i st => do
     let f ← P.receiveChallenge (i.cast hn.symm (cast_symm hSpec)) st
-    return fun chal => f (Challenge.cast_idx hn hSpec ▸ chal)
+    return fun chal => f (Challenge.cast_idx hSpec ▸ chal)
   output := P.output ∘ (fun st => _root_.cast (by simp) st)
 
 @[simp]
@@ -263,15 +288,17 @@ end Verifier
 
 namespace OracleVerifier
 
-open OracleComp Function
+variable [Oₘ₁ : ∀ i, OracleInterface (pSpec₁.Message i)]
+  [Oₘ₂ : ∀ i, OracleInterface (pSpec₂.Message i)]
 
-variable [∀ i, OracleInterface (pSpec₁.Message i)] [∀ i, OracleInterface (pSpec₂.Message i)]
-
+open Function in
 /-- Casting the oracle verifier of a non-oracle reduction across an equality of `ProtocolSpec`s.
 
 TODO: need a cast of the oracle interfaces as well (i.e. the oracle interface instance is not
 necessarily unique for every type) -/
-protected def cast (V : OracleVerifier oSpec StmtIn OStmtIn StmtOut OStmtOut pSpec₁) :
+protected def cast
+    (hOₘ : ∀ i, Oₘ₁ i = dcast (by simp; congr; exact cast_idx hSpec) (Oₘ₂ (i.cast hn hSpec)))
+    (V : OracleVerifier oSpec StmtIn OStmtIn StmtOut OStmtOut pSpec₁) :
     OracleVerifier oSpec StmtIn OStmtIn StmtOut OStmtOut pSpec₂ where
   verify := fun stmt challenges =>
     simulateQ sorry (V.verify stmt (dcast₂ hn.symm (dcast_symm hn hSpec) challenges))
@@ -285,11 +312,13 @@ protected def cast (V : OracleVerifier oSpec StmtIn OStmtIn StmtOut OStmtOut pSp
     rw [this]
     split
     next a b h' => simp [h']
-    next a b h' => simp [h', MessageIdx.cast]; congr; exact (cast_idx hn hSpec).symm
+    next a b h' => simp [h', MessageIdx.cast]; congr; exact (cast_idx hSpec).symm
+
+variable (hOₘ : ∀ i, Oₘ₁ i = dcast (by simp; congr; exact cast_idx hSpec) (Oₘ₂ (i.cast hn hSpec)))
 
 @[simp]
 theorem cast_id :
-    OracleVerifier.cast rfl rfl =
+    OracleVerifier.cast rfl rfl (fun i => rfl) =
       (id : OracleVerifier oSpec StmtIn OStmtIn StmtOut OStmtOut pSpec₁ → _) := by
   sorry
 
@@ -298,6 +327,11 @@ theorem cast_id :
 --     (fun _ pSpec => OracleVerifier oSpec StmtIn OStmtIn StmtOut OStmtOut pSpec) where
 --   dcast₂ := OracleVerifier.cast
 --   dcast₂_id := OracleVerifier.cast_id
+
+@[simp]
+theorem cast_toVerifier (V : OracleVerifier oSpec StmtIn OStmtIn StmtOut OStmtOut pSpec₁) :
+    (OracleVerifier.cast hn hSpec hOₘ V).toVerifier = Verifier.cast hn hSpec V.toVerifier := by
+  sorry
 
 end OracleVerifier
 
@@ -324,18 +358,20 @@ end Reduction
 
 namespace OracleReduction
 
-variable [∀ i, OracleInterface (pSpec₁.Message i)] [∀ i, OracleInterface (pSpec₂.Message i)]
+variable [Oₘ₁ : ∀ i, OracleInterface (pSpec₁.Message i)]
+  [Oₘ₂ : ∀ i, OracleInterface (pSpec₂.Message i)]
+  (hOₘ : ∀ i, Oₘ₁ i = dcast (by simp; congr; exact cast_idx hSpec) (Oₘ₂ (i.cast hn hSpec)))
 
 /-- Casting the oracle reduction across an equality of `ProtocolSpec`s, which casts the underlying
   prover and verifier. -/
 protected def cast (R : OracleReduction oSpec StmtIn OStmtIn WitIn StmtOut OStmtOut WitOut pSpec₁) :
     OracleReduction oSpec StmtIn OStmtIn WitIn StmtOut OStmtOut WitOut pSpec₂ where
   prover := R.prover.cast hn hSpec
-  verifier := R.verifier.cast hn hSpec
+  verifier := R.verifier.cast hn hSpec hOₘ
 
 @[simp]
 theorem cast_id :
-    OracleReduction.cast rfl rfl =
+    OracleReduction.cast rfl rfl (fun _ => rfl) =
       (id : OracleReduction oSpec StmtIn OStmtIn WitIn StmtOut OStmtOut WitOut pSpec₁ → _) := by
   ext : 2 <;> simp [OracleReduction.cast]
 
@@ -347,4 +383,160 @@ theorem cast_id :
 --   dcast₂ := OracleReduction.cast
 --   dcast₂_id := OracleReduction.cast_id
 
+@[simp]
+theorem cast_toReduction
+    (R : OracleReduction oSpec StmtIn OStmtIn WitIn StmtOut OStmtOut WitOut pSpec₁) :
+    (R.cast hn hSpec hOₘ).toReduction = Reduction.cast hn hSpec R.toReduction := by
+  simp [OracleReduction.cast, Reduction.cast, OracleReduction.toReduction, OracleProver.cast]
+
 end OracleReduction
+
+section Execution
+
+-- TODO: show that the execution of everything is the same, modulo casting of transcripts
+variable {pSpec₁ : ProtocolSpec n₁} {pSpec₂ : ProtocolSpec n₂} (hSpec : pSpec₁.cast hn = pSpec₂)
+  [OChal₁ : ∀ i, OracleInterface (pSpec₁.Challenge i)]
+  [OChal₂ : ∀ i, OracleInterface (pSpec₂.Challenge i)]
+  (hOChal : ∀ i, OChal₁ i = dcast (by simp) (OChal₂ (i.cast hn hSpec)))
+
+namespace Prover
+
+-- TODO: need to cast [pSpec₁.Challenge]ₒ to [pSpec₂.Challenge]ₒ
+-- Will not be automatic... require an extra hypothesis
+
+theorem cast_processRound (j : Fin n₁)
+    (P : Prover oSpec StmtIn WitIn StmtOut WitOut pSpec₁)
+    (currentResult : OracleComp (oSpec ++ₒ [pSpec₁.Challenge]ₒ)
+      (Transcript j.castSucc pSpec₁ × P.PrvState j.castSucc)) :
+    P.processRound j currentResult =
+      cast (sorry) ((P.cast hn hSpec).processRound (Fin.cast hn j) sorry) := by
+  sorry
+
+theorem cast_runToRound (j : Fin (n₁ + 1)) (stmt : StmtIn) (wit : WitIn)
+    (P : Prover oSpec StmtIn WitIn StmtOut WitOut pSpec₁) :
+    P.runToRound j stmt wit =
+      cast (sorry) ((P.cast hn hSpec).runToRound (Fin.cast (congrArg (· + 1) hn) j) stmt wit) := by
+  sorry
+
+theorem cast_run (stmt : StmtIn) (wit : WitIn)
+    (P : Prover oSpec StmtIn WitIn StmtOut WitOut pSpec₁) :
+    P.run stmt wit =
+      cast (sorry) ((P.cast hn hSpec).run stmt wit) := by
+  sorry
+
+end Prover
+
+namespace Verifier
+
+variable (V : Verifier oSpec StmtIn StmtOut pSpec₁)
+
+/-- The casted verifier produces the same output as the original verifier. -/
+@[simp]
+theorem cast_run (stmt : StmtIn) (transcript : FullTranscript pSpec₁) :
+    V.run stmt transcript = (V.cast hn hSpec).run stmt (transcript.cast hn hSpec) := by
+  simp only [Verifier.run, Verifier.cast, FullTranscript.cast, dcast₂]
+  unfold Transcript.cast
+  simp
+
+end Verifier
+
+namespace Reduction
+
+variable (R : Reduction oSpec StmtIn WitIn StmtOut WitOut pSpec₁)
+
+theorem cast_run (stmt : StmtIn) (wit : WitIn) :
+    R.run stmt wit = cast (sorry) ((R.cast hn hSpec).run stmt wit) := by
+  sorry
+
+end Reduction
+
+end Execution
+
+section Security
+
+open NNReal
+
+variable {σ : Type} {init : ProbComp σ} {impl : QueryImpl oSpec (StateT σ ProbComp)}
+  [inst₁ : ∀ i, SelectableType (pSpec₁.Challenge i)]
+  [inst₂ : ∀ i, SelectableType (pSpec₂.Challenge i)]
+  (hChallenge : ∀ i, inst₁ i = dcast (by simp) (inst₂ (i.cast hn hSpec)))
+
+section Protocol
+
+variable {relIn : Set (StmtIn × WitIn)} {relOut : Set (StmtOut × WitOut)}
+
+namespace Reduction
+
+variable (R : Reduction oSpec StmtIn WitIn StmtOut WitOut pSpec₁)
+
+@[simp]
+theorem cast_completeness (ε : ℝ≥0) (hComplete : R.completeness init impl relIn relOut ε) :
+    (R.cast hn hSpec).completeness init impl relIn relOut ε := by
+  sorry
+
+@[simp]
+theorem cast_perfectCompleteness (hComplete : R.perfectCompleteness init impl relIn relOut) :
+    (R.cast hn hSpec).perfectCompleteness init impl relIn relOut :=
+  cast_completeness hn hSpec R 0 hComplete
+
+end Reduction
+
+namespace Verifier
+
+variable (V : Verifier oSpec StmtIn StmtOut pSpec₁)
+
+@[simp]
+theorem cast_rbrKnowledgeSoundness (ε : pSpec₁.ChallengeIdx → ℝ≥0)
+    (hRbrKs : V.rbrKnowledgeSoundness init impl relIn relOut ε) :
+    (V.cast hn hSpec).rbrKnowledgeSoundness init impl relIn relOut
+      (ε ∘ (ChallengeIdx.cast hn.symm (cast_symm hSpec))) := by
+  sorry
+
+end Verifier
+
+end Protocol
+
+section OracleProtocol
+
+variable [Oₘ₁ : ∀ i, OracleInterface (pSpec₁.Message i)]
+  [Oₘ₂ : ∀ i, OracleInterface (pSpec₂.Message i)]
+  (hOₘ : ∀ i, Oₘ₁ i = dcast (by simp; congr; exact cast_idx hSpec) (Oₘ₂ (i.cast hn hSpec)))
+  {relIn : Set ((StmtIn × ∀ i, OStmtIn i) × WitIn)}
+  {relOut : Set ((StmtOut × ∀ i, OStmtOut i) × WitOut)}
+
+namespace OracleReduction
+
+variable (R : OracleReduction oSpec StmtIn OStmtIn WitIn StmtOut OStmtOut WitOut pSpec₁)
+
+@[simp]
+theorem cast_completeness (ε : ℝ≥0) (hComplete : R.completeness init impl relIn relOut ε) :
+    (R.cast hn hSpec hOₘ).completeness init impl relIn relOut ε := by
+  unfold completeness
+  rw [cast_toReduction]
+  exact Reduction.cast_completeness hn hSpec R.toReduction ε hComplete
+
+@[simp]
+theorem cast_perfectCompleteness (hComplete : R.perfectCompleteness init impl relIn relOut) :
+    (R.cast hn hSpec hOₘ).perfectCompleteness init impl relIn relOut :=
+  cast_completeness hn hSpec hOₘ R 0 hComplete
+
+end OracleReduction
+
+namespace OracleVerifier
+
+variable (V : OracleVerifier oSpec StmtIn OStmtIn StmtOut OStmtOut pSpec₁)
+
+@[simp]
+theorem cast_rbrKnowledgeSoundness (ε : pSpec₁.ChallengeIdx → ℝ≥0)
+    (hRbrKs : V.rbrKnowledgeSoundness init impl relIn relOut ε) :
+    (V.cast hn hSpec hOₘ).rbrKnowledgeSoundness init impl relIn relOut
+      (ε ∘ (ChallengeIdx.cast hn.symm (cast_symm hSpec))) := by
+  unfold rbrKnowledgeSoundness
+  rw [cast_toVerifier]
+  exact Verifier.cast_rbrKnowledgeSoundness hn hSpec V.toVerifier ε hRbrKs
+
+end OracleVerifier
+
+end OracleProtocol
+
+end Security
